src/mitchell/group_theory/subgroup.lean
@@ -20,15 +20,21 @@ class is_subgroup [group α] (s : set α) : Prop :=
     (one_mem : (1 : α) ∈ s)
     (inv_mem : ∀ {a}, a ∈ s → a⁻¹ ∈ s) 
     (mul_mem : ∀ {a b}, a ∈ s → b ∈ s → a * b ∈ s) 
-                 
+
+class is_normal_subgroup [group α] (s : set α) : Prop :=
+    (subgroup : is_subgroup s)
+    (normal : ∀ n ∈ s, ∀ g : α, g * n * g⁻¹ ∈ s)
+             
 namespace is_subgroup
 
 attribute [simp] is_subgroup.one_mem 
                  is_subgroup.inv_mem 
                  is_subgroup.mul_mem
 
+attribute [instance] is_normal_subgroup.subgroup
+
 -- Subgroup is a group
-instance [group α] {s : set α} [is_subgroup s] : group s :=
+instance subgroup_group [group α] {s : set α} [is_subgroup s] : group s :=
 {   mul := λ ⟨x, hx⟩ ⟨y, hy⟩, ⟨x * y, mul_mem hx hy⟩,
     mul_assoc := λ ⟨x, hx⟩ ⟨y, hy⟩ ⟨z, hz⟩, subtype.eq $ mul_assoc x y z,
     one := ⟨1, one_mem s⟩,
@@ -37,15 +43,61 @@ instance [group α] {s : set α} [is_subgroup s] : group s :=
     inv := λ ⟨x, hx⟩, ⟨x⁻¹, inv_mem hx⟩,
     mul_left_inv := λ ⟨x, hx⟩, subtype.eq $ mul_left_inv x }
 
+-- Normal subgroup properties
+lemma mem_norm_comm [group α] {a b : α} {S : set α} [is_normal_subgroup S] (hab : a * b ∈ S) : b * a ∈ S := 
+    have h : a⁻¹ * (a * b) * a⁻¹⁻¹ ∈ S, from is_normal_subgroup.normal (a * b) hab a⁻¹,
+    by simp at h; exact h
+
 -- Examples of subgroups
 @[simp]
 def trivial [group α] : set α := {1}
 
-instance trivial_in [group α] : is_subgroup (@is_subgroup.trivial α _) :=
-    by split; by simp [trivial] {contextual := tt}
+lemma trivial_in [group α] : is_subgroup (@is_subgroup.trivial α _) :=
+    by split; simp [trivial] {contextual := tt}
+
+lemma univ_in [group α] : is_subgroup (@univ α) :=
+    by split; simp
+
+attribute [instance] trivial_in univ_in
+
+def center (α : Type u) [group α] : set α := {z | ∀ g, g * z = z * g}
+
+lemma center_subg [group α] : is_subgroup (center α) := {
+    is_subgroup .
+    one_mem := by simp [center],
+    mul_mem := begin
+    intros a b ha hb g,
+    rw [center, mem_set_of_eq] at *,
+    rw [←mul_assoc, ha g, mul_assoc, hb g, ←mul_assoc]
+    end,
+    inv_mem := begin
+    assume a ha g,
+    simp [center] at *,
+    calc
+        g * a⁻¹ = a⁻¹ * (g * a) * a⁻¹     : by simp [ha g]
+        ...     = a⁻¹ * g                 : by rw [←mul_assoc, mul_assoc]; simp
+    end
+}
+
+attribute [instance] center_subg
+
+lemma center_normal [group α] : is_normal_subgroup (center α) := {
+    is_normal_subgroup .
+    subgroup := is_subgroup.center_subg,
+    normal := begin
+    simp [center, mem_set_of_eq],
+    intros n ha g h,
+    calc
+        h * (g * n * g⁻¹) = h * n               : by simp [ha g, mul_assoc]
+        ...               = g * g⁻¹ * n * h     : by rw ha h; simp
+        ...               = g * n * g⁻¹ * h     : by rw [mul_assoc g, ha g⁻¹, ←mul_assoc]
+    end
+}
 
 end is_subgroup
 
+
+-- Homomorphism subgroups
 namespace is_hom
 open is_subgroup
 variables [group α] [group β]
@@ -53,7 +105,7 @@ variables [group α] [group β]
 @[simp]
 def kernel {f : α → β} (hf : is_hom f) : set α := preimage f is_subgroup.trivial
 
-instance image_in {f : α → β} (hf: is_hom f) (S : set α) [is_subgroup S] : is_subgroup (f '' S) := {
+lemma image_in {f : α → β} (hf: is_hom f) (S : set α) [is_subgroup S] : is_subgroup (f '' S) := {
     is_subgroup .
     mul_mem := assume a₁ a₂ ⟨b₁, hb₁, eq₁⟩ ⟨b₂, hb₂, eq₂⟩,
     ⟨b₁ * b₂, mul_mem hb₁ hb₂, by simp [eq₁, eq₂, hf.hom_mul]⟩,
@@ -62,18 +114,18 @@ instance image_in {f : α → β} (hf: is_hom f) (S : set α) [is_subgroup S] : 
     ⟨b⁻¹, inv_mem hb, by rw hf.inv; simp *⟩ 
 }
 
-instance preimage_in {f : β → α} (hf : is_hom f) (S : set α) [is_subgroup S] : is_subgroup (f ⁻¹' S) :=
+lemma preimage_in {f : β → α} (hf : is_hom f) (S : set α) [is_subgroup S] : is_subgroup (f ⁻¹' S) :=
     by split; simp [hf.hom_mul, hf.one, hf.inv] {contextual:=tt}
 
-instance kernel_in {f : α → β} (hf: is_hom f) : is_subgroup (hf.kernel) := 
+lemma kernel_in {f : α → β} (hf: is_hom f) : is_subgroup (hf.kernel) := 
     is_hom.preimage_in hf $ trivial
 
-end is_hom
+lemma kernel_normal {f : α → β} (hf: is_hom f) : is_normal_subgroup (hf.kernel) := {
+    normal := by simp [hf.hom_mul, hf.one, hf.inv] {contextual:=tt},
+    subgroup := hf.kernel_in
+}
 
-namespace is_subgroup
-
-section subgroup
-variables [group α] [group β]
+attribute [instance] image_in preimage_in kernel_in kernel_normal
 
 lemma kernel_iff_equiv {f : α → β} (hf: is_hom f) (a b : α) : f b = f a ↔ a⁻¹ * b ∈ hf.kernel :=
 begin
@@ -111,62 +163,4 @@ begin
     }
 end
 
-def center (α : Type u) [group α] : set α := {z | ∀ g, g * z = z * g}
-
-instance center_subg : is_subgroup (center α) := {
-    is_subgroup .
-    one_mem := by simp [center],
-    mul_mem := begin
-    intros a b ha hb g,
-    rw [center, mem_set_of_eq] at *,
-    rw [←mul_assoc, ha g, mul_assoc, hb g, ←mul_assoc]
-    end,
-    inv_mem := begin
-    assume a ha g,
-    simp [center] at *,
-    calc
-        g * a⁻¹ = a⁻¹ * (g * a) * a⁻¹     : by simp [ha g]
-        ...     = a⁻¹ * g                 : by rw [←mul_assoc, mul_assoc]; simp
-    end
-}
-
-end subgroup
-
-class is_normal_subgroup [group α] (s : set α) : Prop :=
-    (subgroup : is_subgroup s)
-    (normal : ∀ n ∈ s, ∀ g : α, g * n * g⁻¹ ∈ s)
-
-section normal_subgroup
-variables [group α] [group β]
-variables {S : set α} [hs : is_normal_subgroup S]
-include hs
-
-attribute [instance] is_normal_subgroup.subgroup
-
-instance kernel_normal {f : α → β} (hf: is_hom f) : is_normal_subgroup (hf.kernel) := {
-    normal := by simp [hf.hom_mul, hf.one, hf.inv] {contextual:=tt},
-    subgroup := hf.kernel_in
-}
-
-instance center_normal : is_normal_subgroup (center α) := {
-    is_normal_subgroup .
-    subgroup := is_subgroup.center_subg,
-    normal := begin
-    simp [center, mem_set_of_eq],
-    intros n ha g h,
-    calc
-        h * (g * n * g⁻¹) = h * n               : by simp [ha g, mul_assoc]
-        ...               = g * g⁻¹ * n * h     : by rw ha h; simp
-        ...               = g * n * g⁻¹ * h     : by rw [mul_assoc g, ha g⁻¹, ←mul_assoc]
-    end
-}
-
--- Normal properties
-
-lemma mem_norm_comm {a b : α} (hab : a * b ∈ S) : b * a ∈ S := 
-    have h : a⁻¹ * (a * b) * a⁻¹⁻¹ ∈ S, from is_normal_subgroup.normal (a * b) hab a⁻¹,
-    by simp at h; exact h
-
-end normal_subgroup
-
-end is_subgroup
+end is_hom
